fixing div

coq/DynamicValue.v
@@ -81,14 +81,14 @@ Definition eval_ibinop_generic {Int} `{VInt Int} `{ConvertToDV Int} (op : ibinop
       else
         to_dvalue res
   | UDiv ex =>
-    if (unsigned x =? 0)%Z then DV_Undef
+    if (unsigned y =? 0)%Z then DV_Undef
     else
       if andb ex (negb ((unsigned x) mod (unsigned y) =? 0)%Z) then
         DV_Poison
       else
         to_dvalue (divu x y)
   | SDiv ex =>
-    if (signed x =? 0)%Z then DV_Undef
+    if (signed y =? 0)%Z then DV_Undef
     else
       if andb ex (negb (((signed x) mod (signed y)) =? 0)%Z) then
         DV_Poison
